do some unfolding in modality tactics

LentilTest/ProofMode/ModalityMisc.lean
@@ -6,6 +6,10 @@ open TLA TLA.ProofMode
 
 variable {σ : Type u} (p q r : pred σ)
 
+def wrappedAlways {α : Type u} (p : pred α) : pred α := [tlafml| □ p]
+
+attribute [tla_modality_unfold] wrappedAlways
+
 example (h : (□ p ∧ □ r) |-tla- (q)) : (□ p ∧ □ r) |-tla- (□ q) := by
   tla_start hp hr
   tla_toggle_goal_under_always
@@ -18,6 +22,25 @@ example (h : (□ p ∧ □ r) |-tla- (□ q)) : (□ p ∧ □ r) |-tla- (q) :=
   tla_toggle_goal_under_always
   tla_toggle_goal_under_always
   tla_check_goal Entails [⟨"hp", [tlafml| □ p]⟩, ⟨"hr", [tlafml| □ r]⟩] [tlafml| □ q]
+  exact h
+
+example (h : (p ⇒ q) |-tla- (r)) : (p ⇒ q) |-tla- (□ r) := by
+  tla_start hp
+  tla_toggle_goal_under_always
+  tla_check_goal Entails [⟨"hp", [tlafml| □ (p → q)]⟩] r
+  exact h
+
+example (h : (wrappedAlways p) |-tla- (r)) : (wrappedAlways p) |-tla- (□ r) := by
+  tla_start hp
+  tla_toggle_goal_under_always
+  tla_check_goal Entails [⟨"hp", [tlafml| □ p]⟩] r
+  exact h
+
+example (h : (p ∧ q) |-tla- (r)) :
+    (wrappedAlways p ∧ wrappedAlways q) |-tla- (wrappedAlways r) := by
+  tla_start hp hq
+  tla_monotone
+  tla_check_goal Entails [⟨"hp", p⟩, ⟨"hq", q⟩] r
   exact h
 
 /--
